lakefile.lean
@@ -5,3 +5,6 @@ package lambdacalc
 
 @[default_target]
 lean_lib LambdaCalc
+
+lean_exe lambdacalc_repl where
+  root := `LambdaCalc.REPL
